type_system/subtyping_lemmas.v
@@ -1,9 +1,9 @@
-(* Add LoadPath "C:\Users\Ziga\Documents\Ziga_podatki\repositories\eeff-formalization\syntax". *)
-(* Add LoadPath "C:\Users\Ziga\Documents\Ziga_podatki\repositories\eeff-formalization\type_system". *)
-(* Add LoadPath "C:\Users\Ziga\Documents\Ziga_podatki\repositories\eeff-formalization\substitution". *)
-Add LoadPath "E:\Ziga_Podatki\faks\eeff-formalization\syntax".
-Add LoadPath "E:\Ziga_Podatki\faks\eeff-formalization\type_system".
-Add LoadPath "E:\Ziga_Podatki\faks\eeff-formalization\substitution".
+Add LoadPath "C:\Users\Ziga\Documents\Ziga_podatki\repositories\eeff-formalization\syntax".
+Add LoadPath "C:\Users\Ziga\Documents\Ziga_podatki\repositories\eeff-formalization\type_system".
+Add LoadPath "C:\Users\Ziga\Documents\Ziga_podatki\repositories\eeff-formalization\substitution".
+(* Add LoadPath "E:\Ziga_Podatki\faks\eeff-formalization\syntax". *)
+(* Add LoadPath "E:\Ziga_Podatki\faks\eeff-formalization\type_system". *)
+(* Add LoadPath "E:\Ziga_Podatki\faks\eeff-formalization\substitution". *)
 
 Require Export declarational wf_lemmas.
 
@@ -280,7 +280,6 @@ revert Γ A i. induction Γ'; intros Γ A i wfg' wfg wfA sty.
     exists (CtxU Γ'' v). exists A'. constructor. rewrite H. f_equal. auto.
     aconstructor. destruct H0. aconstructor. apply SubtypeCtxU; auto.
 Qed.
-
 
 
 Lemma ctx_subtype_remove Γ Γ' i: 
